add negative self comparison example

deps/poulet4/lib/P4automata/Benchmarks/SelfComparison.v
@@ -85,9 +85,9 @@ Module ReadUndef.
   Definition header_eqdec_ (n: nat) (x: header n) (y: header n) : {x = y} + {x <> y}.
     solve_header_eqdec_ n x y 
       [existT (fun n => forall x y: header n, {x = y} + {x <> y}) _ h112_eq_dec;
-       existT (fun n => forall x y: header n, {x = y} + {x <> y}) _ h160_eq_dec;
-       existT (fun n => forall x y: header n, {x = y} + {x <> y}) _ h32_eq_dec;
-       existT (fun n => forall x y: header n, {x = y} + {x <> y}) _ h64_eq_dec].
+       existT _ _ h160_eq_dec;
+       existT _ _ h32_eq_dec;
+       existT _ _ h64_eq_dec].
   Defined. 
 
   Global Instance header_eqdec: forall n, EquivDec.EqDec (header n) eq := header_eqdec_.
@@ -155,3 +155,135 @@ Module ReadUndef.
   Solve Obligations with (destruct s; cbv; Lia.lia).
 
 End ReadUndef.
+
+
+Module ReadUndefIncorrect.
+  Inductive state :=
+  | ParseEth
+  | DefaultVLAN
+  | ParseVLAN
+  | ParseIP
+  | ParseUDP.
+  Scheme Equality for state.
+  Global Instance state_eqdec: EquivDec.EqDec state eq := state_eq_dec.
+  Global Instance state_finite: @Finite state _ state_eq_dec.
+  Proof.
+    solve_finiteness.
+  Qed.
+
+  Inductive header : nat -> Type :=
+  | HdrEth: header eth_size
+  | HdrIP: header ip_size
+  | HdrVLAN: header vlan_size
+  | HdrUDP: header udp_size.
+
+  Derive Signature for header.
+
+  Definition h112_eq_dec (x y: header 112) : {x = y} + {x <> y}.
+    refine (
+        match x, y with 
+        | HdrEth, HdrEth => left eq_refl
+        | _, _ => idProp
+        end);
+      intros H; inversion H.
+  Defined.
+
+  Definition h160_eq_dec (x y: header 160) : {x = y} + {x <> y}.
+    refine (
+        match x, y with 
+        | HdrIP, HdrIP => left eq_refl
+        | _, _ => idProp
+        end);
+      intros H; inversion H.
+  Defined.
+
+  Definition h32_eq_dec (x y: header 32) : {x = y} + {x <> y}.
+    refine (
+        match x, y with 
+        | HdrVLAN, HdrVLAN => left eq_refl
+        | _, _ => idProp
+        end);
+      intros H; inversion H.
+  Defined.
+
+  Definition h64_eq_dec (x y: header 64) : {x = y} + {x <> y}.
+    refine (
+        match x, y with 
+        | HdrUDP, HdrUDP => left eq_refl
+        | _, _ => idProp
+        end);
+      intros H; inversion H.
+  Defined.
+
+  Definition header_eqdec_ (n: nat) (x: header n) (y: header n) : {x = y} + {x <> y}.
+    solve_header_eqdec_ n x y 
+      [existT (fun n => forall x y: header n, {x = y} + {x <> y}) _ h112_eq_dec;
+       existT _ _ h160_eq_dec;
+       existT _ _ h32_eq_dec;
+       existT _ _ h64_eq_dec].
+  Defined. 
+
+  Global Instance header_eqdec: forall n, EquivDec.EqDec (header n) eq := header_eqdec_.
+
+  Global Instance header_eqdec': EquivDec.EqDec (H' header) eq.
+  Proof.
+    solve_eqdec'.
+  Qed.
+
+  Global Instance header_finite: forall n, @Finite (header n) _ _.
+  Proof.
+    intros n; solve_indexed_finiteness n [eth_size;ip_size;vlan_size;udp_size].
+  Qed.
+  Global Program Instance header_finite': @Finite {n & header n} _ header_eqdec' :=
+    {| enum := [ existT _ _ HdrEth ;
+                 existT _ _ HdrIP ;
+                 existT _ _ HdrVLAN ;
+                 existT _ _ HdrUDP ] |}.
+  Next Obligation.
+    solve_header_finite.
+  Qed.
+  Next Obligation.
+  dependent destruction X; subst;
+  repeat (
+    match goal with
+    | |- ?L \/ ?R => (now left; trivial) || right
+    end
+  ).
+  Qed.
+
+  Definition states (s: state) : P4A.state state header :=
+    match s with
+    | ParseEth =>
+      {| st_op := extract(HdrEth);
+         st_trans := transition select (| (EHdr HdrEth)[0 -- 0] |) {{
+                                    [| exact #b|0 |] ==> inl DefaultVLAN ;;;
+                                    [| exact #b|1 |] ==> inl ParseVLAN ;;;
+                                    reject
+                                }}
+      |}
+    | DefaultVLAN =>
+      {| st_op := extract(HdrIP);
+         st_trans := transition (inl ParseUDP)
+      |}
+    | ParseIP =>
+      {| st_op := extract(HdrIP);
+         st_trans := transition (inl ParseUDP)
+      |}
+    | ParseVLAN =>
+      {| st_op := extract(HdrVLAN);
+         st_trans := transition (inl ParseIP)
+      |}
+    | ParseUDP =>
+      {| st_op := extract(HdrUDP);
+         st_trans := transition select (| (EHdr HdrVLAN)[3--0] |) {{
+                                    [| exact #b|1|1|1|1 |] ==> reject ;;;
+                                    accept
+                                }}
+      |}
+    end.
+
+  Program Definition aut: Syntax.t state _ :=
+    {| t_states := states |}.
+  Solve Obligations with (destruct s; cbv; Lia.lia).
+
+End ReadUndefIncorrect.
