deps/poulet4/lib/P4automata/Benchmarks/SelfComparisonProof.v
@@ -1,56 +1,119 @@
 Require Import Poulet4.P4automata.Benchmarks.ProofHeader.
 Require Import Poulet4.P4automata.Benchmarks.SelfComparison.
 
-Notation H := (ReadUndef.header + ReadUndef.header).
-Notation A := (Sum.sum ReadUndef.aut ReadUndef.aut).
-Notation conf := (P4automaton.configuration (P4A.interp A)).
-Definition r_states :=
-  Eval vm_compute in (Reachability.reachable_states
-                        A
-                        10
-                        ReadUndef.ParseEth
-                        ReadUndef.ParseEth).
-
-Definition top : Relations.rel conf := fun _ _ => True.
-Definition top' : Relations.rel (state_template A) := fun _ _ => True.
 
 Declare ML Module "mirrorsolve".
 
-RegisterEnvCtors
-  (ReadUndef.HdrEth, FirstOrderConfRelSimplified.Bits eth_size)
-  (ReadUndef.HdrIP, FirstOrderConfRelSimplified.Bits ip_size)
-  (ReadUndef.HdrVLAN, FirstOrderConfRelSimplified.Bits vlan_size)
-  (ReadUndef.HdrUDP, FirstOrderConfRelSimplified.Bits udp_size).
+Module Positive.
+    
+  Notation H := (ReadUndef.header + ReadUndef.header).
+  Notation A := (Sum.sum ReadUndef.aut ReadUndef.aut).
+  Notation conf := (P4automaton.configuration (P4A.interp A)).
+  Definition r_states :=
+    Eval vm_compute in (Reachability.reachable_states
+                          A
+                          10
+                          ReadUndef.ParseEth
+                          ReadUndef.ParseEth).
 
-Lemma prebisim_babyip:
-  forall q1 q2,
-    interp_conf_rel' {| cr_st := {|
-                        cs_st1 := {|
-                          st_state := inl (inl (ReadUndef.ParseEth));
-                          st_buf_len := 0;
+  Definition top : Relations.rel conf := fun _ _ => True.
+  Definition top' : Relations.rel (state_template A) := fun _ _ => True.
+
+  ClearEnvCtors.
+
+  RegisterEnvCtors
+    (ReadUndef.HdrEth, FirstOrderConfRelSimplified.Bits eth_size)
+    (ReadUndef.HdrIP, FirstOrderConfRelSimplified.Bits ip_size)
+    (ReadUndef.HdrVLAN, FirstOrderConfRelSimplified.Bits vlan_size)
+    (ReadUndef.HdrUDP, FirstOrderConfRelSimplified.Bits udp_size).
+
+  Lemma prebisim_babyip:
+    forall q1 q2,
+      interp_conf_rel' {| cr_st := {|
+                          cs_st1 := {|
+                            st_state := inl (inl (ReadUndef.ParseEth));
+                            st_buf_len := 0;
+                          |};
+                          cs_st2 := {|
+                            st_state := inl (inr (ReadUndef.ParseEth));
+                            st_buf_len := 0;
+                          |};
                         |};
-                        cs_st2 := {|
-                          st_state := inl (inr (ReadUndef.ParseEth));
-                          st_buf_len := 0;
+                        cr_ctx := BCEmp;
+                        cr_rel := btrue;
+                    |} q1 q2 ->
+    pre_bisimulation A
+                    (wp r_states)
+                    top
+                    []
+                    (mk_init _ _ _ A 10 ReadUndef.ParseEth ReadUndef.ParseEth)
+                    q1 q2.
+  Proof.
+    idtac "running self-comparison positive bisimulation".
+
+    intros.
+    set (rel0 := (mk_init _ _ _ A 10 ReadUndef.ParseEth ReadUndef.ParseEth)).
+    vm_compute in rel0.
+    subst rel0.
+
+    time "build phase" repeat (time "single step" run_bisim top top' r_states).
+    time "close phase" close_bisim top'.
+  Time Admitted.
+End Positive.
+
+Module Negative.
+    
+  Notation H := (ReadUndefIncorrect.header + ReadUndefIncorrect.header).
+  Notation A := (Sum.sum ReadUndefIncorrect.aut ReadUndefIncorrect.aut).
+  Notation conf := (P4automaton.configuration (P4A.interp A)).
+  Definition r_states :=
+    Eval vm_compute in (Reachability.reachable_states
+                          A
+                          10
+                          ReadUndefIncorrect.ParseEth
+                          ReadUndefIncorrect.ParseEth).
+
+  Definition top : Relations.rel conf := fun _ _ => True.
+  Definition top' : Relations.rel (state_template A) := fun _ _ => True.
+
+  ClearEnvCtors.
+
+  RegisterEnvCtors
+    (ReadUndefIncorrect.HdrEth, FirstOrderConfRelSimplified.Bits eth_size)
+    (ReadUndefIncorrect.HdrIP, FirstOrderConfRelSimplified.Bits ip_size)
+    (ReadUndefIncorrect.HdrVLAN, FirstOrderConfRelSimplified.Bits vlan_size)
+    (ReadUndefIncorrect.HdrUDP, FirstOrderConfRelSimplified.Bits udp_size).
+
+  Lemma prebisim_babyip:
+    forall q1 q2,
+      interp_conf_rel' {| cr_st := {|
+                          cs_st1 := {|
+                            st_state := inl (inl (ReadUndefIncorrect.ParseEth));
+                            st_buf_len := 0;
+                          |};
+                          cs_st2 := {|
+                            st_state := inl (inr (ReadUndefIncorrect.ParseEth));
+                            st_buf_len := 0;
+                          |};
                         |};
-                      |};
-                      cr_ctx := BCEmp;
-                      cr_rel := btrue;
-                   |} q1 q2 ->
-  pre_bisimulation A
-                   (wp r_states)
-                   top
-                   []
-                   (mk_init _ _ _ A 10 ReadUndef.ParseEth ReadUndef.ParseEth)
-                   q1 q2.
-Proof.
-  idtac "running self-comparison bisimulation".
+                        cr_ctx := BCEmp;
+                        cr_rel := btrue;
+                    |} q1 q2 ->
+    pre_bisimulation A
+                    (wp r_states)
+                    top
+                    []
+                    (mk_init _ _ _ A 10 ReadUndefIncorrect.ParseEth ReadUndefIncorrect.ParseEth)
+                    q1 q2.
+  Proof.
+    idtac "running self-comparison negative bisimulation".
 
-  intros.
-  set (rel0 := (mk_init _ _ _ A 10 ReadUndef.ParseEth ReadUndef.ParseEth)).
-  vm_compute in rel0.
-  subst rel0.
+    intros.
+    set (rel0 := (mk_init _ _ _ A 10 ReadUndefIncorrect.ParseEth ReadUndefIncorrect.ParseEth)).
+    vm_compute in rel0.
+    subst rel0.
 
-  time "build phase" repeat (time "single step" run_bisim top top' r_states).
-  time "close phase" close_bisim top'.
-Time Admitted.
+    time "build phase" repeat (time "single step" run_bisim top top' r_states).
+    Fail time "close phase" close_bisim top'.
+  Time Admitted.
+End Negative.
